compiler,proof: give field names in deep embedding struct constructor

cogent/isa/Cogent.thy
@@ -319,7 +319,7 @@ datatype 'f expr = Var index
                  | Prim prim_op "'f expr list"
                  | App "'f expr" "'f expr"
                  | Con "(name \<times> type \<times> variant_state) list" name "'f expr"
-                 | Struct "type list" "'f expr list"
+                 | Struct "name list" "type list" "'f expr list"
                  | Member "'f expr" field
                  | Unit
                  | Lit lit
@@ -536,7 +536,7 @@ fun specialise :: "type substitution \<Rightarrow> 'f expr \<Rightarrow> 'f expr
 | "specialise \<delta> (Prim p es)       = Prim p (map (specialise \<delta>) es)"
 | "specialise \<delta> (App a b)         = App (specialise \<delta> a) (specialise \<delta> b)"
 | "specialise \<delta> (Con as t e)      = Con (map (\<lambda> (c,t,b). (c, instantiate \<delta> t, b)) as) t (specialise \<delta> e)"
-| "specialise \<delta> (Struct ts vs)    = Struct (map (instantiate \<delta>) ts) (map (specialise \<delta>) vs)"
+| "specialise \<delta> (Struct ns ts vs) = Struct ns (map (instantiate \<delta>) ts) (map (specialise \<delta>) vs)"
 | "specialise \<delta> (Member v f)      = Member (specialise \<delta> v) f"
 | "specialise \<delta> (Unit)            = Unit"
 | "specialise \<delta> (Cast t e)        = Cast t (specialise \<delta> e)"
@@ -862,8 +862,9 @@ typing_var    : "\<lbrakk> K \<turnstile> \<Gamma> \<leadsto>w singleton (length
 | typing_struct : "\<lbrakk> \<Xi>, K, \<Gamma> \<turnstile>* es : ts
                    ; distinct ns
                    ; length ns = length ts
-                   ; ts' = zip ns (zip ts (replicate (length ts) Present))
-                   \<rbrakk> \<Longrightarrow> \<Xi>, K, \<Gamma> \<turnstile> Struct ts es : TRecord ts' Unboxed"
+                   ; ts' = map (\<lambda>(n,t). (n,t,Present)) (zip ns ts)
+                   ; ts'' = ts
+                   \<rbrakk> \<Longrightarrow> \<Xi>, K, \<Gamma> \<turnstile> Struct ns ts'' es : TRecord ts' Unboxed"
 
 | typing_member : "\<lbrakk> \<Xi>, K, \<Gamma> \<turnstile> e : TRecord ts s
                    ; K \<turnstile> TRecord (ts[f := (n, t, Taken)]) s :\<kappa> k
@@ -921,7 +922,7 @@ inductive_cases typing_caseE   [elim]: "\<Xi>, K, \<Gamma> \<turnstile> Case x t
 inductive_cases typing_esacE   [elim]: "\<Xi>, K, \<Gamma> \<turnstile> Esac e t : \<tau>"
 inductive_cases typing_castE   [elim]: "\<Xi>, K, \<Gamma> \<turnstile> Cast t e : \<tau>"
 inductive_cases typing_letE    [elim]: "\<Xi>, K, \<Gamma> \<turnstile> Let a b : \<tau>"
-inductive_cases typing_structE [elim]: "\<Xi>, K, \<Gamma> \<turnstile> Struct ts es : \<tau>"
+inductive_cases typing_structE [elim]: "\<Xi>, K, \<Gamma> \<turnstile> Struct ns ts es : \<tau>"
 inductive_cases typing_letbE   [elim]: "\<Xi>, K, \<Gamma> \<turnstile> LetBang vs a b : \<tau>"
 inductive_cases typing_takeE   [elim]: "\<Xi>, K, \<Gamma> \<turnstile> Take x f e : \<tau>"
 inductive_cases typing_putE    [elim]: "\<Xi>, K, \<Gamma> \<turnstile> Put x f e : \<tau>"
@@ -940,7 +941,7 @@ inductive atom ::"'f expr \<Rightarrow> bool" where
 | "atom (AFun f ts)"
 | "atom (Prim p (map Var is))"
 | "atom (Con ts n (Var x))"
-| "atom (Struct ts (map Var is))"
+| "atom (Struct ns ts (map Var is))"
 | "atom (Cast t (Var x))"
 | "atom (Member (Var x) f)"
 | "atom Unit"
@@ -1868,8 +1869,8 @@ lemma specialise_eq_convs:
   "\<And>us a b.     App a b         = specialise us x \<longleftrightarrow> (\<exists>a' b'. x = App a' b' \<and> a = specialise us a' \<and> b = specialise us b')"
   "\<And>us as t e.  Con as t e      = specialise us x \<longleftrightarrow>
                   (\<exists>as' e'. x = Con as' t e' \<and> as = map (\<lambda>(c,t,b). (c, instantiate us t, b)) as' \<and> e = specialise us e')"
-  "\<And>us ts vs.   Struct ts vs    = specialise us x \<longleftrightarrow>
-                  (\<exists>ts' vs'. x = Struct ts' vs' \<and> ts = map (instantiate us) ts' \<and> vs = map (specialise us) vs')"
+  "\<And>ns us ts vs. Struct ns ts vs = specialise us x \<longleftrightarrow>
+                  (\<exists>ts' vs'. x = Struct ns ts' vs' \<and> ts = map (instantiate us) ts' \<and> vs = map (specialise us) vs')"
   "\<And>us v f.     Member v f      = specialise us x \<longleftrightarrow> (\<exists>v'. x = Member v' f \<and> v = specialise us v')"
   "\<And>us.         Unit            = specialise us x \<longleftrightarrow> x = Unit"
   "\<And>us t e.     Cast t e        = specialise us x \<longleftrightarrow> (\<exists>e'. x = Cast t e' \<and> e = specialise us e')"
@@ -2382,7 +2383,8 @@ next case typing_fun then show ?case
     by (clarsimp simp add: kinding_defs instantiate_wellformed list_all2_kinding_wellformedD list_all2_lengthD)
 next case typing_esac then show ?case
     by (fastforce dest: filter_member2  simp add: kinding_simps kinding_variant_set list_all_iff)
-next case typing_struct then show ?case by (clarsimp simp add: in_set_zip list_all_iff)
+next case typing_struct then show ?case
+    by (simp add: list_all_zip_iff_list_all2 list_all2_conv_all_nth list_all_length)
 next case typing_member then show ?case
     by (fastforce simp add: kinding_defs INT_subset_iff list_all_iff dest: nth_mem split: prod.splits record_state.splits)
 next case typing_put then show ?case
@@ -2512,7 +2514,7 @@ fun expr_size :: "'f expr \<Rightarrow> nat" where
 | "expr_size (Prim p as) = Suc (sum_list (map expr_size as))"
 | "expr_size (Var v) = 0"
 | "expr_size (AFun v va) = 0"
-| "expr_size (Struct v va) = Suc (sum_list (map expr_size va))"
+| "expr_size (Struct ns v va) = Suc (sum_list (map expr_size va))"
 | "expr_size (Lit v) = 0"
 | "expr_size (SLit s) = 0"
 | "expr_size (Tuple v va) = Suc ((expr_size v) + (expr_size va))"
